theories/MemClient.v
@@ -22,12 +22,47 @@ Section PROOF.
   Context `{@GRA.inG memRA Σ}.
 
   Definition MemMain1: Mod.t := Mod.add Mem Main.
-  Definition MemMain2: Mod.t := Mod.add Mem Main.
+
+  Definition MainSem2: ModSem.t := {|
+    ModSem.fnsems := List.map (map_snd fun_to_src) MainStb;
+    ModSem.initial_mrs := [("Main", ε)];
+  |}
+  .
+
+  Definition Main2: Mod.t := {|
+    Mod.get_modsem := fun _ => MainSem2;
+    (* Mod.sk := List.map fst MainStb; *)
+    Mod.sk := Sk.unit;
+  |}
+  .
+
+  Definition MemSem2: ModSem.t := {|
+    ModSem.fnsems := List.map (map_snd fun_to_src) MemStb;
+    ModSem.initial_mrs := [("Mem", ε)];
+  |}
+  .
+
+  Definition Mem2: Mod.t := {|
+    Mod.get_modsem := fun _ => MemSem2; (*** TODO: we need proper handling of function pointers ***)
+    (* Mod.sk := List.map fst MemStb; *)
+    Mod.sk := Sk.unit;
+  |}
+  .
+
+  Definition MemMain2: Mod.t := Mod.add Mem2 Main2.
+
+  Theorem correct: Beh.of_program (Mod.interp MemMain1) <1= Beh.of_program (Mod.interp MemMain2).
+  Proof.
+    ii.
+    set (global_stb:=MemStb++MainStb).
+    (* clearbody global_stb. *)
+    Local Opaque MemStb.
+    Local Opaque Mem1.MemStb.
+    Local Opaque MainStb.
+    eapply adequacy_type with (stb:=global_stb) in PR. cbn in *.
+    rp; try apply PR; cycle 1.
+    { refl. }
+    clear PR. f_equal.
+  Qed.
 
 End PROOF.
-
-
-
-
-
-
